CancelIL, but it doesn't depend on IL.

src/CancelIL.v
@@ -1,7 +1,5 @@
 Require Import List.
 Require Import IL SepIL.
-Require Import Word Memory.
-Require Import DepList EqdepClass.
 Require Import Expr SepExpr SepCancel.
 Require Import Prover.
 Require Import Tactics Reflection.
@@ -10,643 +8,240 @@ Require ExprUnify.
 Set Implicit Arguments.
 Set Strict Implicit.
 
-Module U := ExprUnify.UNIFIER.
-Module CANCEL := SepCancel.Make U SepIL.SH.
+Require UnfolderTac CancelTac.
 
-Section existsSubst.
-  Variable types : list type.
-  Variable funcs : functions types.
-  Variable meta_base : env types.
-  Variable var_env : env types.
-  Variable sub : U.Subst types.
- 
-  Definition ExistsSubstNone (_ : tvar) (_ : expr types) := 
-    False.
+Module SE := SepExpr.Make SepIL.ST.
+Module SH := SepHeap.Make SE.
 
-  Fixpoint substInEnv (from : nat) (vals : env types) (ret : env types -> Prop) : Prop :=
-    match vals with 
-      | nil => ret nil
-      | val :: vals =>
-        match U.Subst_lookup from sub with
-          | None => substInEnv (S from) vals (fun e => ret (val :: e))
-          | Some v => 
-            match exprD funcs meta_base var_env v (projT1 val) with
-              | None => ExistsSubstNone (projT1 val) v
-              | Some v' => projT2 val = v' /\ substInEnv (S from) vals (fun e => ret (existT _ (projT1 val) v' :: e))
-            end
-        end
+Module UNF := Unfolder.Make SH ExprUnify.UNIFIER.
+Module UNF_TAC := UnfolderTac.UnfolderTac UNF.
+
+Module CANCEL := SepCancel.Make ExprUnify.UNIFIER SH.
+Module CANCEL_TAC := CancelTac.CancellerTac CANCEL.
+
+Section parametric.
+  Variable ts : list type.
+  Variable tpreds : SE.tpredicates.
+  Variable prover : ProverT ts.
+  
+  Inductive cancelResult : Type :=
+  | Done : forall (lhs rhs : SH.SHeap ts), cancelResult
+  | Quant : forall (alls : list tvar) (pures : exprs ts) (exs : list tvar) (sub : ExprUnify.UNIFIER.Subst ts),
+    cancelResult -> cancelResult.
+
+  Variable fs : functions ts.
+  Variable ps : SE.predicates ts.
+
+  Fixpoint cancelResultD (U G : env ts) (cr : cancelResult) {struct cr} : Prop :=
+    match cr with
+      | Done l r =>
+        (** TODO: Should I perform the substitution now? *)
+        AllProvable_and fs U G 
+          (SE.himp fs ps U G (SH.sheapD l) 
+                             (SH.sheapD (SH.Build_SHeap (SH.impures r) nil (SH.other r))))
+          (SH.pures r)
+      | Quant alls pures exs sub r =>
+        forallEach alls (fun Aext => 
+          let G := G ++ Aext in
+          AllProvable_impl fs U G
+            (@CANCEL_TAC.existsSubst ts fs G sub 0 
+              (map (fun x => @existT _ (fun tv => option (tvarD ts tv)) (projT1 x) (Some (projT2 x))) U ++
+               map (fun x => @existT _ _ x None) exs)
+              (fun U => cancelResultD U G r))
+          pures)
     end.
 
-  Fixpoint existsMaybe (vals : list { t : tvar & option (tvarD types t) }) (ret : env types -> Prop) : Prop :=
-    match vals with
-      | nil => ret nil
-      | existT t None :: vals => exists x : tvarD types t, existsMaybe vals (fun e => ret (existT _ t x :: e))
-      | existT t (Some v) :: vals => existsMaybe vals (fun e => ret (existT _ t v :: e))
+  Require Import Bool.
+
+  Variables hintsFwd hintsBwd : UNF.hintSide ts.
+
+  (** This will implement a loop of unfolding and cancellation **)
+  Fixpoint cancelLoop (n : nat) (facts : Facts prover) (uvars vars : list tvar)
+    (l r : SH.SHeap ts) (sub : ExprUnify.UNIFIER.Subst ts) (prog : bool) {struct n}
+    : cancelResult * bool :=
+    match n with 
+      | 0 => 
+        let Lhs' := SH.Build_SHeap (SH.impures l) nil (SH.other l) in
+        (Quant nil (SH.pures l) nil sub (Done Lhs' r), true)
+      | S n =>
+        (** Start by doing refinement **)
+        let '(unf, prog') := @UNF_TAC.unfold ts prover facts hintsFwd hintsBwd uvars vars l r in
+        @UNF_TAC.unfolderResult_rect ts prover _ 
+          (fun alls exs lhs rhs know =>
+            let '(cncl, prog'') := @CANCEL_TAC.canceller ts prover tpreds know lhs rhs sub in
+            if prog' || prog'' then
+              match cncl with
+                | {| CANCEL_TAC.Lhs := Lhs; CANCEL_TAC.Rhs := Rhs; CANCEL_TAC.Subst := Subst |} =>
+                  let Lhs' := SH.Build_SHeap (SH.impures Lhs) nil (SH.other Lhs) in
+                  let '(res, p) := cancelLoop n know (uvars ++ exs) (vars ++ alls) Lhs' Rhs Subst true in
+                  (Quant alls (SH.pures Lhs) exs Subst res, p)
+              end
+            else
+              (Done l r, prog))
+          unf
     end.
 
-End existsSubst.
+End parametric.
 
-Definition existsSubst types funcs var_env sub (from : nat) (vals : list { t : tvar & option (tvarD types t) }) (ret : env types -> Prop) :=
-  existsMaybe vals (fun e => @substInEnv types funcs e var_env sub from e ret).
-
-Fixpoint consistent {ts} (vals : list { x : tvar & option (tvarD ts x) }) (e : list { x : tvar & tvarD ts x }) : Prop :=
-  match vals , e with
-    | nil , nil => True
-    | existT t None :: vals , existT t' _ :: e =>
-      t = t' /\ @consistent _ vals e
-    | existT t (Some v) :: vals , existT t' v' :: e =>
-      match equiv_dec t t' return Prop with
-        | left pf => 
-          v' = match (pf : t = t') in _ = t return tvarD ts t with
-                 | refl_equal => v
-               end /\ @consistent _ vals e
-        | right _ => False
-      end
-    | _ , _ => False
-  end.
-
-Lemma ex_iff : forall T (P P' : T -> Prop),
-  (forall x, P x <-> P' x) ->
-  ((exists x, P x) <-> (exists x, P' x)).
-Proof. split; intuition; destruct H0 as [ x ? ]; exists x; firstorder. Qed.
-
-Theorem existsMaybe_sem : forall types vals (ret : env types -> Prop),
-  existsMaybe vals ret <->
-  existsEach (map (@projT1 _ _) vals) (fun e => consistent vals e /\ ret e).
+Theorem AllProvable_impl_sem : forall ts (funcs : functions ts)  U G P ps,
+  AllProvable_impl funcs U G P ps <-> (AllProvable funcs U G ps -> P).
 Proof.
-  induction vals; simpl; intros.
-  { intuition. }
-  { destruct a. destruct o.
-    { rewrite IHvals. intuition. exists t. apply existsEach_sem. apply existsEach_sem in H.
-      destruct H. exists x0. simpl in *. rewrite EquivDec_refl_left. intuition.
-      destruct H. apply existsEach_sem. apply existsEach_sem in H. destruct H.
-      exists x1. simpl in *. rewrite EquivDec_refl_left in H. intuition; subst; auto. }
-    { simpl. eapply ex_iff. intros. rewrite IHvals.
-      intuition; apply existsEach_sem in H; apply existsEach_sem; destruct H; exists x1; intuition. } }
+  induction ps; simpl in *; unfold Basics.impl; intuition.
 Qed.
 
-Lemma substInEnv_sem : forall types funcs meta_env var_env sub vals from ret,
-  @substInEnv types funcs meta_env var_env sub from vals ret <-> 
-  (U.Subst_equations_to funcs meta_env var_env sub from vals /\ ret vals).
+Lemma cancelLoop_ind_pf : forall 
+  types (funcs : functions types) (preds : SE.predicates types) 
+  prover hintsFwd hintsBwd
+  (bound : nat) uvars vars (lhs rhs : SH.SHeap types) (facts : Facts prover) sub_init
+  cr prog b,
+  forall (PC : ProverT_correct prover funcs),
+  UNF.SH.WellTyped_sheap (typeof_funcs funcs) (UNF.SH.SE.typeof_preds preds)
+    (typeof_env uvars) (typeof_env vars) rhs = true ->
+  CANCEL.U.Subst_equations funcs uvars vars sub_init ->
+  Valid PC uvars vars facts ->
+  UNF.hintSideD funcs preds hintsFwd ->
+  UNF.hintSideD funcs preds hintsBwd ->
+  cancelLoop (SE.typeof_preds preds) prover hintsFwd hintsBwd bound facts (typeof_env uvars) (typeof_env vars) lhs rhs
+    sub_init b = (cr, prog) ->
+  (cancelResultD funcs preds uvars vars cr) ->
+  SE.himp funcs preds uvars vars (SH.sheapD lhs) (SH.sheapD rhs).
 Proof.
-  induction vals; simpl; intros.
-  { intuition. }
-  { destruct a; simpl in *.
-    consider (U.Subst_lookup from sub); simpl; intros.
-    consider (exprD funcs meta_env var_env e x); simpl; intros.
-    { rewrite IHvals. intuition; subst; auto. } 
-    { intuition. }
-    { rewrite IHvals. intuition. } }
-Qed.
-
-Lemma existsSubst_sem : forall ts (funcs : functions ts) vals sub vars_env from ret,
-  existsSubst funcs vars_env sub from vals ret <->
-  existsEach (map (@projT1 _ _) vals) (fun meta_env =>
-    consistent vals meta_env /\ U.Subst_equations_to funcs meta_env vars_env sub from meta_env /\ ret meta_env).
-Proof.
-  intros. unfold existsSubst.
-  rewrite existsMaybe_sem. rewrite existsEach_sem. rewrite existsEach_sem.
-  apply ex_iff. intros. rewrite substInEnv_sem. intuition.
-Qed.
-
-Lemma AllProvable_impl_AllProvable : forall ts (funcs : functions ts) U G P ps,
-  AllProvable funcs U G ps ->
-  AllProvable_impl funcs U G P ps ->
-  P.
-Proof. clear. induction ps; simpl; intros; eauto. intuition. Qed.    
-
-Section canceller.
-  Variable types : list type.
-  Variable funcs : functions types.
-  Variable preds : SEP.predicates types.
-  Variable prover : ProverT types.
-  Variable hints : option hintSide.
-
-  Variable algos : ILAlgoTypes.AllAlgos ts.
-
-  Record CancellerResult : Type :=
-  { AllExt : variables
-  ; ExExt  : variables
-  ; Lhs    : SH.SHeap types BedrockCoreEnv.pc BedrockCoreEnv.st
-  ; Rhs    : SH.SHeap types BedrockCoreEnv.pc BedrockCoreEnv.st
-  ; Subst  : U.Subst types
-  }.
-
-  Definition canceller (uvars : list tvar) (hyps : Expr.exprs types)
-    (lhs rhs : SEP.sexpr types BedrockCoreEnv.pc BedrockCoreEnv.st) : option CancellerResult :=
-    let prover := 
-      match ILAlgoTypes.Prover algos with
-        | None => provers.ReflexivityProver.reflexivityProver
-        | Some p => p
-      end
-    in
-    let hints :=
-      match ILAlgoTypes.Hints algos with
-        | None => UNF.default_hintsPayload _ _ _ 
-        | Some h => h
-      end
-    in
-    let (ql, lhs) := SH.hash lhs in
-    let facts := Summarize prover (map (liftExpr 0 0 0 (length ql)) hyps ++ SH.pures lhs) in
-    let pre :=
-      {| UNF.Vars  := rev ql
-       ; UNF.UVars := uvars
-       ; UNF.Heap  := lhs
-      |}
-    in
-    match UNF.forward hints prover 10 facts pre with
-      | ({| UNF.Vars := vars' ; UNF.UVars := uvars' ; UNF.Heap := lhs |}, n_forward) =>
-        let (qr, rhs) := SH.hash rhs in
-        let rhs :=
-          UNF.HEAP_FACTS.sheapSubstU 0 (length qr) (length uvars') rhs
-        in
-        let post :=
-          {| UNF.Vars  := vars'
-           ; UNF.UVars := uvars' ++ rev qr
-           ; UNF.Heap  := rhs
-          |}
-        in
-        match UNF.backward hints prover 10 facts post with
-          | ({| UNF.Vars := vars' ; UNF.UVars := uvars' ; UNF.Heap := rhs |}, n_backward) =>
-            let new_vars  := vars' in
-            let new_uvars := skipn (length uvars) uvars' in
-            let bound := length uvars' in
-            match CANCEL.sepCancel preds prover bound facts lhs rhs (U.Subst_empty _) false with
-              | Some (l,r,s) =>
-                Some {| AllExt := new_vars
-                      ; ExExt  := new_uvars
-                      ; Lhs    := 
-                        (** TODO: this is a hack for the moment to ensure that
-                         ** the pure premises are well typed without the new
-                         ** unification variables
-                         **)
-                        {| SH.impures := SH.impures l
-                         ; SH.pures   := SH.pures lhs
-                         ; SH.other   := SH.other l
-                         |}
-                      ; Rhs    := r
-                      ; Subst  := s
-                      |}
-              | None => 
-                if match ql , qr with
-                     | nil , nil =>
-                       match SH.pures lhs , SH.pures rhs with
-                         | nil, nil => 
-                           if EqNat.beq_nat n_forward 10 then EqNat.beq_nat n_backward 10 else false
-                         | _ , _ => false
-                       end
-                     | _ , _ => false 
-                   end then
-                  None
-                else 
-                  Some {| AllExt := new_vars
-                        ; ExExt  := new_uvars
-                        ; Lhs    := lhs
-                        ; Rhs    := rhs
-                        ; Subst  := U.Subst_empty _
-                        |}
-            end
-        end
-    end.
-
-  Lemma AllProvable_and_sem : forall U G P Ps,
-    AllProvable_and funcs U G P Ps <-> (AllProvable funcs U G Ps /\ P).
-  Proof. induction Ps; simpl; intros; intuition auto. Qed.
-  Lemma app_inj_length : forall T (a b c d : list T),
-    a ++ b = c ++ d ->
-    length a = length c ->
-    a = c /\ b = d.
-  Proof.
-    induction a; destruct c; simpl; intros; think; try solve [ intuition ].
-    inversion H; subst.  eapply IHa in H3. intuition; subst; auto. omega.
-  Qed.
-  Lemma WellTyped_env_app : forall ts a b c d,
-    WellTyped_env a c ->
-    WellTyped_env b d ->
-    WellTyped_env (types := ts) (a ++ b) (c ++ d).
-  Proof. clear.
-    intros. unfold WellTyped_env in *. unfold typeof_env in *. subst. 
-    rewrite map_app. reflexivity.
-  Qed.
-  Ltac t_list_length := repeat (rewrite typeof_env_length || rewrite rev_length || rewrite map_length || rewrite app_length).
-  Hint Extern 1 (_ = _) => t_list_length; auto : list_length.
-
-  Ltac env_resolution :=
-    repeat (rewrite typeof_env_app || unfold typeof_env || rewrite map_app || rewrite map_rev || (f_equal; []) || assumption).
-
-  Lemma consistent_app : forall ts a b c,
-    consistent (ts := ts) (a ++ b) c ->
-    consistent a (firstn (length a) c) /\ consistent b (skipn (length a) c).
-  Proof. clear.
-    induction a; simpl; intros; auto.
-    destruct a. destruct o. destruct c; try contradiction. destruct s. destruct (equiv_dec x x0); try contradiction.
-    destruct H. eapply IHa in H0. intuition.
-    destruct c; try contradiction. destruct s. destruct H. apply IHa in H0. intuition.
-  Qed.
-  Lemma consistent_Some : forall ts a c,
-    consistent (ts := ts) (map (fun x => existT _ (projT1 x) (Some (projT2 x))) a) c ->
-    a = c.
-  Proof.
-    induction a; destruct c; simpl; intros; try contradiction; auto.
-    destruct s. destruct a; simpl in *. destruct (equiv_dec x0 x); try contradiction.
-    unfold equiv in e. intuition; subst. f_equal; eauto.
-  Qed.
-  Lemma skipn_length : forall T a (b : list T),
-    length (skipn a b) = length b - a.
-  Proof. induction a; destruct b; simpl; intros; auto. Qed.
-
-  Lemma himp_remove_pure_p : forall cs U G p P Q,
-    (Provable funcs U G p ->
-      SH.SE.himp funcs preds U G cs P Q) ->
-    SH.SE.himp funcs preds U G cs (SEP.Star (@SEP.Inj _ _ _ p) P) Q.
-  Proof. clear.
-    intros. unfold SH.SE.himp. simpl. unfold Provable in *. 
-    destruct (exprD funcs U G p tvProp); eapply himp_star_pure_c; intuition.
-  Qed.
-  Lemma himp_remove_pures_p : forall cs U G ps P Q,
-    (AllProvable funcs U G ps ->
-      SH.SE.himp funcs preds U G cs P Q) ->
-    SH.SE.himp funcs preds U G cs (SH.starred (@SEP.Inj _ _ _) ps P) Q.
-  Proof. clear.
-    induction ps; intros.
-    { rewrite SH.starred_nil. apply H. exact I. }
-    { rewrite SH.starred_cons. apply himp_remove_pure_p. intros.
-      eapply IHps. intro. apply H; simpl; auto. }
-  Qed.
-  Lemma himp_remove_pure_c : forall cs U G p P Q,
-    Provable funcs U G p ->
-    SH.SE.himp funcs preds U G cs P Q ->
-    SH.SE.himp funcs preds U G cs P (SEP.Star (@SEP.Inj _ _ _ p) Q).
-  Proof. clear.
-    intros. unfold SH.SE.himp. simpl. unfold Provable in *. 
-    destruct (exprD funcs U G p tvProp); eapply himp_star_pure_cc; intuition.
-  Qed.
-  Lemma himp_remove_pures_c : forall cs U G ps P Q,
-    AllProvable funcs U G ps ->
-    SH.SE.himp funcs preds U G cs P Q ->
-    SH.SE.himp funcs preds U G cs P (SH.starred (@SEP.Inj _ _ _) ps Q).
-  Proof. clear.
-    induction ps; intros.
-    { rewrite SH.starred_nil. apply H0. }
-    { rewrite SH.starred_cons. simpl in *. apply himp_remove_pure_c; intuition. }
-  Qed.
-
-  Lemma ApplyCancelSep_with_eq' : 
-    forall (algos_correct : ILAlgoTypes.AllAlgos_correct funcs preds algos),
-    forall (meta_env : env types) (hyps : Expr.exprs types),
-    Expr.AllProvable funcs meta_env nil hyps ->
-    forall (l r : SEP.sexpr types BedrockCoreEnv.pc BedrockCoreEnv.st) res cs,
-    forall (WTR : SEP.WellTyped_sexpr (typeof_funcs funcs) (SEP.typeof_preds preds) (typeof_env meta_env) nil r = true),
-    canceller (typeof_env meta_env) hyps l r = Some res ->
-    match res with
-      | {| AllExt := new_vars
-         ; ExExt  := new_uvars
-         ; Lhs    := lhs'
-         ; Rhs    := rhs'
-         ; Subst  := subst
-         |} =>
-        Expr.forallEach new_vars (fun nvs : Expr.env types =>
-          let var_env := nvs in
-          Expr.AllProvable_impl funcs meta_env var_env
-          (existsSubst funcs var_env subst 0 
-            (map (fun x => existT (fun t => option (tvarD types t)) (projT1 x) (Some (projT2 x))) meta_env ++
-             map (fun x => existT (fun t => option (tvarD types t)) x None) new_uvars)
-            (fun meta_env : Expr.env types =>
-                (Expr.AllProvable_and funcs meta_env var_env
-                  (himp cs 
-                    (SEP.sexprD funcs preds meta_env var_env
-                      (SH.sheapD (SH.Build_SHeap _ _ (SH.impures lhs') nil (SH.other lhs'))))
-                    (SEP.sexprD funcs preds meta_env var_env
-                      (SH.sheapD (SH.Build_SHeap _ _ (SH.impures rhs') nil (SH.other rhs')))))
-                  (SH.pures rhs')) ))
-            (SH.pures lhs'))
-    end ->
-    himp cs (@SEP.sexprD _ _ _ funcs preds meta_env nil l)
-            (@SEP.sexprD _ _ _ funcs preds meta_env nil r).
-  Proof.
-    Opaque UNF.backward UNF.forward Env.repr.
-    intros. unfold canceller in *.
-    assert (PC : ProverT_correct
-              match ILAlgoTypes.Prover algos with
-              | Some p => p
-              | None => ReflexivityProver.reflexivityProver
-              end funcs).
-    { generalize (ILAlgoTypes.Acorrect_Prover algos_correct).
-      destruct (ILAlgoTypes.Prover algos); intros; auto.
-      apply ReflexivityProver.reflexivityProver_correct. }
-    generalize dependent (match ILAlgoTypes.Prover algos with
-                            | Some p => p
-                            | None => ReflexivityProver.reflexivityProver
-                          end).
-    match goal with
-      | [ |- context [ ?X ] ] =>
-        match X with 
-          | match ILAlgoTypes.Hints _ with _ => _ end =>
-            assert (HC : UNF.hintsSoundness funcs preds X); [ | generalize dependent X ]
-        end
-    end.
-    { generalize (ILAlgoTypes.Acorrect_Hints algos_correct).     
-      destruct (ILAlgoTypes.Hints algos); auto using UNF.hintsSoundness_default. }
-    intros h HC p ? PC.
-    consider (SH.hash l); intros.
-    rewrite SH.hash_denote. rewrite H0; clear H0; simpl.
-    consider (SH.hash r); intros.
-    rewrite SH.hash_denote with (s := r). rewrite H0; simpl.
-    rewrite UNF.himp_existsEach_ST_EXT_existsEach.
-    rewrite UNF.ST_EXT.himp_existsEach_p; [ reflexivity | intros ].
-    rewrite app_nil_r.
-    apply CANCEL.HEAP_FACTS.himp_pull_pures; intro.
-    match goal with 
-      | [ H : context [ Summarize ?P ?ps ] |- _ ] =>
-        assert (Valid PC meta_env (rev G) (Summarize P ps)); [ | generalize dependent (Summarize P ps); intros ]
-    end.
-    { eapply Summarize_correct.
-      apply AllProvable_app; auto.
-      revert H; clear - H3. induction hyps; simpl; intros; auto.
-      intuition. clear - H0 H3. unfold Provable in *.
-      generalize (liftExpr_ext funcs meta_env nil nil nil (rev G) nil a tvProp); simpl.
-      rewrite app_nil_r. rewrite rev_length. subst. rewrite map_length.
-      intro. rewrite H in *. auto. }
-    match goal with
-      | [ H : match ?X with _ => _ end = _ |- _ ] => consider X
-    end; intros.
-    apply CANCEL.SEP_FACTS.himp_WellTyped_sexpr; intro.
-
-    (** Forward **)
-    destruct (UNF.forwardLength _ _ _ _ _ H2).
-    assert (SH.WellTyped_sheap (typeof_funcs funcs) (UNF.SE.typeof_preds preds) (typeof_env meta_env) (rev v) s = true).
-    { rewrite SH.WellTyped_sheap_WellTyped_sexpr. rewrite <- H3. rewrite <- map_rev. apply H7. }
-(*
-    generalize (@UNF.forward_WellTyped _ _ _ _ _ _ _ HC _ _ _ _ H2 H9); intro.
+  induction bound; simpl; intros.
+  { inversion H4; clear H4; subst.
     simpl in *.
-    assert (WellTyped_env (rev v) (rev G)).
-    { unfold WellTyped_env. subst. rewrite <- map_rev. auto. }
-    eapply UNF.forwardOk  with (cs := cs) in H2; simpl; eauto using typeof_env_WellTyped_env.
-    simpl in H2. etransitivity; [ eapply H2 | clear H11; simpl in * ].
-    rewrite UNF.ST_EXT.himp_existsEach_p; [ reflexivity | intros ].
-    destruct H8.
-    (** NOTE: I can't shift s0 around until I can witness the existential **)
-    
-    (** Open up everything **)
-    consider (UNF.backward h p 10 f
-           {| UNF.Vars := Vars
-            ; UNF.UVars := UVars ++ rev v0
-            ; UNF.Heap := UNF.HEAP_FACTS.sheapSubstU 0 (length v0) (length UVars) s0 |}); intros.
-    destruct (UNF.backwardLength _ _ _ _ _ H6); simpl in *.
-    consider (CANCEL.sepCancel preds p (length UVars0) f Heap Heap0 (U.Subst_empty _)); intros; try congruence.
-    destruct p0. destruct p0. inversion H15; clear H15; subst. intuition; subst.
-    rewrite ListFacts.rw_skipn_app in H11 by auto with list_length. 
+    eapply UNF.HEAP_FACTS.himp_pull_pures; intros.
+    repeat rewrite app_nil_r in *.
+    eapply AllProvable_impl_AllProvable in H5; eauto.
+    eapply CANCEL_TAC.existsSubst_sem in H5.
+    rewrite map_map in *; simpl in *.
+    eapply existsEach_sem in H5. destruct H5. intuition.
+    eapply CANCEL_TAC.consistent_Some in H5. subst.
+    eapply AllProvable_and_sem in H9. intuition.
+    eapply UNF_TAC.SH_UTIL.sheapD_remove_pures_p.
+    eapply UNF_TAC.SH_UTIL.sheapD_remove_pures_c; eauto. }
+  { consider (UNF_TAC.unfold prover facts hintsFwd hintsBwd 
+              (typeof_env uvars) (typeof_env vars) lhs rhs); intros.
+    destruct u; simpl in *.
+    consider (CANCEL_TAC.canceller prover (SE.typeof_preds preds) Know Lhs Rhs sub_init); intros.
+    destruct (b0 || b1).
+    { destruct c.
+      match goal with
+        | [ H : match ?X with _ => _ end = _ |- _ ] =>
+          consider X
+      end; intros.
+      inversion H8; clear H8; subst.
+      simpl in *.
+      eapply CANCEL_TAC.SH_FACTS.SEP_FACTS.himp_WellTyped_sexpr; intro.
+      eapply UNF_TAC.ApplyUnfold_with_eq' in H4; try eassumption. intros.
+      eapply forallEach_sem; intros.
 
-    eapply forallEach_sem with (env := rev G ++ G0) in H1; [ | solve [ env_resolution ] ]. 
+      eapply AllProvable_impl_sem; intros.
+      generalize (CANCEL_TAC.canceller_PuresPrem _ _ _ _ _ _ _ _ _ H6 H13). simpl; intro.
 
-    eapply (@CANCEL.HEAP_FACTS.himp_pull_pures types _ _ funcs preds cs meta_env (rev G ++ G0) Heap). intro.
-    eapply AllProvable_impl_AllProvable in H1; [ clear H3 | assumption ].
-   
-    apply existsSubst_sem in H1. apply existsEach_sem in H1.
-    destruct H1. intuition.
-    assert (meta_env = firstn (length meta_env) x1 /\
-            typeof_env (skipn (length (rev v0)) (skipn (length meta_env) x1)) = x0 /\ 
-            typeof_env (firstn (length (rev v0)) (skipn (length meta_env) x1)) = rev v0).
-    { clear - H3 H1.
-      generalize (typeof_env_length x1). rewrite H3; intros.
-      rewrite <- firstn_skipn with (n := length meta_env) (l := x1) in H3.
-      repeat (rewrite map_app in *  || rewrite map_map in * || rewrite map_id in * || rewrite app_ass in *
-        || rewrite ListFacts.rw_skipn_app in * by eauto || rewrite typeof_env_app in * ).
-      simpl in *. rewrite typeof_env_app in *. eapply app_inj_length in H3.
-      Focus 2. revert H. t_list_length. rewrite firstn_length. intro. rewrite min_l; omega.
-      destruct H3.
-      rewrite <- firstn_skipn with (n := length (rev v0)) (l := skipn (length meta_env) x1) in H2.
-      rewrite typeof_env_app in *. 
-      eapply app_inj_length in H2. destruct H2. intuition.
-      { eapply consistent_app in H1. destruct H1; clear - H1.
-        revert H1. t_list_length. intros.
-        eapply consistent_Some in H1. auto. }
-      revert H. t_list_length. intro. rewrite firstn_length; rewrite min_l; auto.
-      rewrite skipn_length. omega. }
-    intuition. clear H3 H1.
+      eapply forallEach_sem in H5; try eassumption.
+      eapply AllProvable_impl_sem in H5; try eassumption.
+      eapply CANCEL_TAC.existsSubst_sem in H5.
+      eapply existsEach_sem in H5. destruct H5; intuition.
 
-    eapply AllProvable_and_sem in H14. destruct H14.
-    rewrite app_ass in *.
+      eapply UNF.ST_EXT.himp_existsEach_c.
+      eapply CANCEL_TAC.consistent_app in H5. intuition.
+      rewrite map_length in *.
+      rewrite map_app in *; repeat rewrite map_map in *; simpl in *.
+      rewrite map_id in *. exists (skipn (length uvars) x).
+      rewrite <- firstn_skipn with (l := x) (n := length uvars) in H15.
+      unfold typeof_env in H15; rewrite map_app in H15.
+      eapply ListFacts.app_inj_length in H15.
+      intuition.
 
-    assert (SH.WellTyped_sheap (typeof_funcs funcs) (UNF.SE.typeof_preds preds)
-     (typeof_env meta_env ++ rev v0)
-     (rev (map (projT1 (P:=tvarD types)) G) ++ x)
-     (UNF.HEAP_FACTS.sheapSubstU 0 (length v0) (length (typeof_env meta_env))
-        s0) = true).
-    { rewrite <- SH.WellTyped_sheap_WellTyped_sexpr in H7.
-      generalize (@UNF.HEAP_FACTS.sheapSubstU_WellTyped types BedrockCoreEnv.pc BedrockCoreEnv.st (typeof_funcs funcs) (UNF.SE.typeof_preds preds) (typeof_env meta_env) nil (rev v0) nil s0); simpl.   
-      rewrite app_nil_r. intro XX.
-      rewrite SH.WellTyped_hash in WTR. rewrite H0 in WTR. simpl in WTR. rewrite app_nil_r in WTR.
-      apply XX in WTR. clear XX.
-      eapply SH.WellTyped_sheap_weaken with (tU' := nil) (tG := nil) (tG' := (rev (map (projT1 (P:=tvarD types)) G) ++ x)) in WTR. 
-      simpl in WTR. rewrite app_nil_r in WTR.  
-      rewrite Plus.plus_0_r in *. rewrite rev_length in WTR. apply WTR. }
-    
-    generalize (@UNF.backward_WellTyped _ _ _ _ _ _ _ HC _ _ _ _ H6 H14); simpl.
-    eapply UNF.backwardOk with (cs := cs) in H6; simpl in *.
-    2: eassumption.
-    2: solve [ rewrite <- H17; eapply WellTyped_env_app; eauto using typeof_env_WellTyped_env ].
-    Focus 2.
-    rewrite <- map_rev.
-    eapply WellTyped_env_app. eapply typeof_env_WellTyped_env.
-    instantiate (1 := G0). symmetry. apply H11. 
-    2: eassumption.
-    2: solve [ eapply Valid_weaken; eassumption ].
-    intro.
+      eapply CANCEL_TAC.ApplyCancelSep_with_eq' with (funcs := funcs)
+        (meta_env := (uvars ++ skipn (length uvars) x)) (var_env := var_env) in H6.
+      intuition.
+      rewrite <- H6.
+      eapply UNF_TAC.SH_UTIL.sheapD_remove_pures_c.
+      rewrite <- app_nil_r with (l := var_env). eapply AllProvable_weaken. eassumption.
+      rewrite <- app_nil_r with (l := var_env) at 2.
+      eapply UNF.HEAP_FACTS.SEP_FACTS.sexprD_weaken.
+      rewrite <- app_nil_r with (l := var_env). eapply Valid_weaken. eassumption.
+      subst var_env.
+      eapply CANCEL_TAC.consistent_Some in H17. rewrite H17.
+      rewrite <- H17 at 2. rewrite firstn_skipn.
 
-    (** **)
-    rewrite UNF.himp_existsEach_ST_EXT_existsEach.
-    eapply UNF.ST_EXT.himp_existsEach_c. exists (rev (firstn (length (rev v0)) (skipn (length meta_env) x1))); split.
-    { rewrite map_rev. unfold typeof_env in H17. rewrite H17. apply rev_involutive. }
-    rewrite rev_involutive.
-    
-    (** In order to call the canceller, they must have the same environments. **)
-    assert (SH.SE.ST.heq cs 
-              (SH.SE.sexprD funcs preds meta_env (rev G ++ G0) (SH.sheapD Heap))
-              (SH.SE.sexprD funcs preds x1 (rev G ++ G0) (SH.sheapD Heap))).
-    { rewrite <- firstn_skipn with (l := x1) (n := length meta_env).
-      rewrite <- H15.
-      generalize (@CANCEL.SEP_FACTS.sexprD_weaken_wt types _ _ funcs preds cs meta_env (skipn (length meta_env) x1) nil 
-        (SH.sheapD Heap) (rev G ++ G0)).
-      rewrite app_nil_r. intro XX; apply XX; clear XX.
-      rewrite <- SH.WellTyped_sheap_WellTyped_sexpr. rewrite <- H10. f_equal.
-      rewrite typeof_env_app. f_equal. rewrite <- map_rev. reflexivity.
-      rewrite <- H11. reflexivity. }
-    etransitivity; [ eapply H18 | clear H18 ].
+      { clear - H0 H17. 
+        rewrite <- firstn_skipn with (l := x) (n := length uvars).        
+        simpl in *. cutrewrite (firstn (length uvars) x ++ skipn (length uvars) x = uvars ++ skipn (length uvars) x).
+        eapply ExprUnify.UNIFIER.Subst_equations_weaken; eauto.
+        f_equal. symmetry. apply H17. }
 
-    assert (SH.SE.ST.heq cs 
-              (SH.SE.sexprD funcs preds (meta_env ++ firstn (length (rev v0)) (skipn (length meta_env) x1)) (rev G ++ G0) (SH.sheapD (UNF.HEAP_FACTS.sheapSubstU 0 (length v0)
-                       (length (typeof_env meta_env)) s0)))
-              (UNF.SE.sexprD funcs preds meta_env
-                (firstn (length (rev v0)) (skipn (length meta_env) x1) ++ nil)
-                (SH.sheapD s0))).
-    { generalize (@UNF.HEAP_FACTS.sheapSubstU_sheapD types _ _ funcs preds cs 
-        meta_env nil (firstn (length (rev v0)) (skipn (length meta_env) x1)) nil s0).
-      simpl. repeat rewrite app_nil_r. intros XX; rewrite XX; clear XX.
-      generalize (@CANCEL.SEP_FACTS.sexprD_weaken_wt types _ _ funcs preds cs
-        (meta_env ++ firstn (length (rev v0)) (skipn (length meta_env) x1))
-        nil (rev G ++ G0)
-          (SH.sheapD (UNF.HEAP_FACTS.sheapSubstU 0
-              (length (firstn (length (rev v0)) (skipn (length meta_env) x1)) +
-               0) (length meta_env) s0)) nil).
-      simpl. t_list_length.
-      intro XX; rewrite XX; clear XX.
-      rewrite H15. rewrite app_ass. 
-      cutrewrite (length (firstn (length meta_env) x1) = length meta_env).
-      rewrite app_nil_r.
-      cutrewrite (length (firstn (length v0) (skipn (length meta_env) x1)) + 0 = length v0).
-      reflexivity.
-      rewrite Plus.plus_0_r. rewrite <- rev_length with (l := v0). 
-      rewrite <- H17 at 2. t_list_length. reflexivity.
-      rewrite <- H15. reflexivity.
-      rewrite <- SH.WellTyped_sheap_WellTyped_sexpr.
-      rewrite SH.WellTyped_hash in WTR.
-      rewrite SH.WellTyped_sheap_WellTyped_sexpr in WTR. rewrite H0 in *. simpl in WTR.
-      clear - WTR H15 H12 H17 H11.
-      rewrite <- SH.WellTyped_sheap_WellTyped_sexpr in WTR.
-      generalize (@UNF.HEAP_FACTS.sheapSubstU_WellTyped_eq types BedrockCoreEnv.pc BedrockCoreEnv.st (typeof_funcs funcs) (SEP.typeof_preds preds)
-        (typeof_env meta_env) nil (rev v0) nil s0). simpl. t_list_length. rewrite app_nil_r in *.
-      intro XX; rewrite XX in WTR; clear XX.
-      rewrite <- WTR. rewrite <- H17. t_list_length. rewrite typeof_env_app. repeat rewrite Plus.plus_0_r.
-      f_equal. f_equal. rewrite <- rev_length with (l := v0). rewrite <- H17 at 2.
-      t_list_length. reflexivity. }
-    rewrite <- H18; clear H18.
-    revert H6. t_list_length.
-    intro H6. etransitivity; [ clear H6 | eapply H6 ].
+      unfold typeof_env in *. rewrite map_app. rewrite H20.
+      unfold var_env. rewrite map_app. rewrite H11.
+      eassumption.
 
-    
-    (** witness the conclusion **)
-    eapply UNF.ST_EXT.himp_existsEach_c. 
-    exists (skipn (length (rev v0)) (skipn (length meta_env) x1)). split. 
-    { t_list_length. rewrite firstn_length; rewrite skipn_length. rewrite <- app_ass. rewrite ListFacts.rw_skipn_app.
-      rewrite <- H12. t_list_length. reflexivity.
-      env_resolution. t_list_length. f_equal. rewrite min_l; auto.
-      clear - H17 H15 H12.
-      assert (x1 = firstn (length meta_env) x1 ++ (firstn (length (rev v0)) (skipn (length meta_env) x1)) ++ 
-        (skipn (length (rev v0)) (skipn (length meta_env) x1))).
-      repeat rewrite firstn_skipn. reflexivity. 
-      generalize dependent (firstn (length meta_env) x1).
-      generalize dependent (skipn (length (rev v0)) (skipn (length meta_env) x1)).
-      generalize dependent (firstn (length (rev v0)) (skipn (length meta_env) x1)).
-      intros. subst. rewrite <- rev_length. rewrite <- H17. t_list_length. omega. }
-    rewrite app_ass. rewrite H15 at 1.
-    t_list_length. repeat rewrite firstn_skipn.
-    clear H2. 
+      unfold typeof_env in *. rewrite map_app. rewrite H20.
+      unfold var_env. rewrite map_app. rewrite H11.
+      rewrite SH.WellTyped_sheap_WellTyped_sexpr. 
+      rewrite <- app_nil_r with (l := map (projT1 (P:=tvarD types)) vars ++ Alls).
+      eapply UNF.HEAP_FACTS.SEP_FACTS.WellTyped_sexpr_weaken.
+      rewrite <- SH.WellTyped_sheap_WellTyped_sexpr. eassumption.
 
-    (** Finally the cancellation **)
-    assert (U.Subst_WellTyped (typeof_funcs funcs) (typeof_env x1)
-      (typeof_env (rev G ++ G0)) (U.Subst_empty types)).
-    { eapply U.Subst_empty_WellTyped. }
-    assert (SH.WellTyped_sheap (typeof_funcs funcs) (CANCEL.SE.typeof_preds preds)
-      (typeof_env x1) (typeof_env (rev G ++ G0)) Heap0 = true).
-    { rewrite <- H16. f_equal.
-      rewrite H15. rewrite <- H17. rewrite <- H12. t_list_length. 
-      repeat rewrite <- typeof_env_app. repeat rewrite firstn_skipn. reflexivity.
-      rewrite typeof_env_app. f_equal. rewrite typeof_env_rev. reflexivity. apply H11. }
-    assert (SH.WellTyped_sheap (typeof_funcs funcs) (CANCEL.SE.typeof_preds preds)
-     (typeof_env x1) (typeof_env (rev G ++ G0)) Heap = true).
-    { eapply SH.WellTyped_sheap_weaken with (tG' := nil) (tU' := typeof_env (skipn (length meta_env) x1)) in H10.
-      rewrite H15 in H10 at 1. rewrite <- typeof_env_app in H10. rewrite firstn_skipn in H10.
-      rewrite app_nil_r in H10. rewrite <- H10. f_equal.
-      rewrite typeof_env_app. rewrite typeof_env_rev. f_equal. apply H11. }
-    eapply CANCEL.sepCancel_correct with (cs := cs) (funcs := funcs) (U := x1) (G := rev G ++ G0) in H13; try eassumption.
-    { instantiate (1 := PC). eapply Valid_weaken with (ue := skipn (length meta_env) x1) (ge := G0) in H5.
-      rewrite <- firstn_skipn with (n := length meta_env) (l := x1). rewrite <- H15. assumption. }
-    { (* eapply CANCEL.sepCancel_PuresPrem in H13; try eassumption. *)
-      match type of H3 with
-        | himp ?CS (SEP.sexprD ?F ?P ?U ?G ?L) (SEP.sexprD ?F ?P ?U ?G ?R) =>
-          change (SEP.himp F P U G CS L R) in H3
-      end. 
-      do 2 rewrite SH.sheapD_def. do 2 rewrite SH.sheapD_def in H3. simpl in *.
-      do 2 rewrite CANCEL.SEP_FACTS.heq_star_emp_l in H3.
-      rewrite CANCEL.SEP_FACTS.heq_star_comm 
-        with (P := SH.starred (SEP.Inj (stateType:=BedrockCoreEnv.st)) (SH.pures s2) SEP.Emp).
-      rewrite CANCEL.SEP_FACTS.heq_star_comm 
-        with (P := SH.starred (SEP.Inj (stateType:=BedrockCoreEnv.st)) (SH.pures s3) SEP.Emp).
-      do 2 rewrite <- CANCEL.SEP_FACTS.heq_star_assoc.
-      apply CANCEL.SEP_FACTS.himp_star_frame. assumption.
-      eapply himp_remove_pures_p; intros.
-      eapply himp_remove_pures_c; auto. reflexivity. } 
-    { eapply CANCEL.sepCancel_PureFacts in H13. 4: eapply H6. 
-      eapply U.Subst_equations_to_Subst_equations; intuition.
-      intuition. intuition. }
-  Qed.
-*)
-  Admitted.
+      rewrite <- H20 in H7. rewrite <- H11 in H7.
+      change (map (projT1 (P:=tvarD types)) (skipn (length uvars) x)) with (typeof_env (skipn (length uvars) x)) in H7.
+      repeat rewrite <- typeof_env_app in H7.
 
-  Lemma ApplyCancelSep_with_eq : 
-    forall (algos_correct : ILAlgoTypes.AllAlgos_correct funcs preds algos),
-    forall (meta_env : env (Env.repr BedrockCoreEnv.core types)) (hyps : Expr.exprs (_)),
+      simpl; intros.
+      eapply IHbound in H7; try eassumption.
+      { simpl; intros. 
+        eapply CANCEL_TAC.existsSubst_sem.
+        rewrite map_map. simpl.
+        eapply existsEach_sem.
+        exists (uvars ++ skipn (length uvars) x).
+        { intuition.
+          eapply CANCEL_TAC.consistent_Some; reflexivity.
+          { assert (x = uvars ++ skipn (length uvars) x).
+            { rewrite <- firstn_skipn with (l := x) (n := length uvars) at 1.
+              f_equal. eapply CANCEL_TAC.consistent_Some in H17. auto. }
+            rewrite <- H23 in *. eassumption. }
+          unfold SE.himp in H7.
+          subst var_env. rewrite <- H7.
+          eapply UNF_TAC.SH_UTIL.sheapD_remove_pures_p. reflexivity. } }
+      { assert (x = uvars ++ skipn (length uvars) x).
+        { rewrite <- firstn_skipn with (l := x) (n := length uvars) at 1.
+          f_equal. eapply CANCEL_TAC.consistent_Some in H17. auto. }
+        rewrite <- H23 in *.
+        eapply CANCEL.U.Subst_equations_to_Subst_equations; eauto.
+        eapply CANCEL_TAC.canceller_PureFacts in H6.
+        simpl in *. intuition. eapply H24.
+        rewrite H23. 
+        eapply CANCEL.U.Subst_equations_weaken in H0.
+        eapply CANCEL.U.Subst_equations_WellTyped in H0.
+        eassumption.
 
-    forall (l r : SEP.sexpr types BedrockCoreEnv.pc BedrockCoreEnv.st) res,
-    canceller (typeof_env meta_env) hyps l r = Some res ->
-    Expr.AllProvable funcs meta_env nil hyps ->
-    forall (WTR : SEP.WellTyped_sexpr (typeof_funcs funcs) (SEP.typeof_preds preds) (typeof_env meta_env) nil r = true) cs,
+        rewrite H23. rewrite <- H11 in *. repeat rewrite typeof_env_app.
+        rewrite <- app_nil_r with (l := typeof_env vars ++ typeof_env env).
+        repeat rewrite SH.WellTyped_sheap_WellTyped_sexpr in *.
+        rewrite UNF.HEAP_FACTS.SEP_FACTS.WellTyped_sexpr_weaken by eassumption. reflexivity.
 
-    match res with
-      | {| AllExt := new_vars
-         ; ExExt  := new_uvars
-         ; Lhs    := lhs'
-         ; Rhs    := rhs'
-         ; Subst  := subst
-         |} =>
-        Expr.forallEach new_vars (fun nvs : Expr.env types =>
-          let var_env := nvs in
-          Expr.AllProvable_impl funcs meta_env var_env
-          (existsSubst funcs var_env subst 0 
-            (map (fun x => existT (fun t => option (tvarD types t)) (projT1 x) (Some (projT2 x))) meta_env ++
-             map (fun x => existT (fun t => option (tvarD types t)) x None) new_uvars)
-            (fun meta_env : Expr.env types =>
-                (Expr.AllProvable_and funcs meta_env var_env
-                  (himp cs 
-                    (SEP.sexprD funcs preds meta_env var_env
-                      (SH.sheapD (SH.Build_SHeap _ _ (SH.impures lhs') nil (SH.other lhs'))))
-                    (SEP.sexprD funcs preds meta_env var_env
-                      (SH.sheapD (SH.Build_SHeap _ _ (SH.impures rhs') nil (SH.other rhs')))))
-                  (SH.pures rhs')) ))
-            (SH.pures lhs'))
-    end ->
-    himp cs (@SEP.sexprD _ _ _ funcs preds meta_env nil l)
-            (@SEP.sexprD _ _ _ funcs preds meta_env nil r).
-  Proof. intros. eapply ApplyCancelSep_with_eq'; eauto. Qed.
+        rewrite H23. rewrite <- H11 in *. rewrite <- H20 in *. repeat rewrite typeof_env_app.
+        repeat rewrite SH.WellTyped_sheap_WellTyped_sexpr in *.
+        unfold typeof_env in *. eassumption. }
 
-  Lemma ApplyCancelSep : 
-    forall (algos_correct : ILAlgoTypes.AllAlgos_correct funcs preds algos),
-    forall (meta_env : env (Env.repr BedrockCoreEnv.core types)) (hyps : Expr.exprs (_)),
-    forall (l r : SEP.sexpr types BedrockCoreEnv.pc BedrockCoreEnv.st),
-      Expr.AllProvable funcs meta_env nil hyps ->
-    forall (WTR : SEP.WellTyped_sexpr (typeof_funcs funcs) (SEP.typeof_preds preds) (typeof_env meta_env) nil r = true) cs,
-    match canceller (typeof_env meta_env) hyps l r with
-      | Some {| AllExt := new_vars
-         ; ExExt  := new_uvars
-         ; Lhs    := lhs'
-         ; Rhs    := rhs'
-         ; Subst  := subst
-         |} =>
-        Expr.forallEach new_vars (fun nvs : Expr.env types =>
-          let var_env := nvs in
-          Expr.AllProvable_impl funcs meta_env var_env
-          (existsSubst funcs var_env subst 0 
-            (map (fun x => existT (fun t => option (tvarD types t)) (projT1 x) (Some (projT2 x))) meta_env ++
-             map (fun x => existT (fun t => option (tvarD types t)) x None) new_uvars)
-            (fun meta_env : Expr.env types =>
-                (Expr.AllProvable_and funcs meta_env var_env
-                  (himp cs 
-                    (SEP.sexprD funcs preds meta_env var_env
-                      (SH.sheapD (SH.Build_SHeap _ _ (SH.impures lhs') nil (SH.other lhs'))))
-                    (SEP.sexprD funcs preds meta_env var_env
-                      (SH.sheapD (SH.Build_SHeap _ _ (SH.impures rhs') nil (SH.other rhs')))))
-                  (SH.pures rhs')) ))
-            (SH.pures lhs'))
-      | None => 
-        himp cs (@SEP.sexprD _ _ _ funcs preds meta_env nil l)
-                (@SEP.sexprD _ _ _ funcs preds meta_env nil r)
-    end ->
-    himp cs (@SEP.sexprD _ _ _ funcs preds meta_env nil l)
-            (@SEP.sexprD _ _ _ funcs preds meta_env nil r).
-  Proof. 
-    intros. consider (canceller (typeof_env meta_env) hyps l r); intros; auto.
-    eapply ApplyCancelSep_with_eq; eauto.
-  Qed.
+      rewrite <- app_nil_r with (l := vars ++ env).
+      eapply Valid_weaken; eauto.
 
-End canceller.
+      eapply CANCEL_TAC.consistent_Some in H17.
+      rewrite H17 at 1. rewrite firstn_skipn. eassumption. 
+
+      repeat rewrite map_length. rewrite firstn_length.
+      rewrite Min.min_l; auto.
+      clear - H15.
+      rewrite <- map_app in H15. rewrite firstn_skipn in H15.
+      assert (length (map (projT1 (P:=tvarD types)) x) =
+        length (map (fun x : sigT (tvarD types) => projT1 x) uvars ++ Exs)).
+      { rewrite H15; auto. }
+      repeat rewrite map_length in *. rewrite app_length in *.
+      rewrite map_length in *. omega. }
+    { inversion H7; clear H7; subst. simpl in *.
+      eapply AllProvable_and_sem in H5. destruct H5.
+      eapply UNF_TAC.SH_UTIL.sheapD_remove_pures_c; eauto. } }
+Qed.
+
+
